

# Supplementary material for Lesson 4

## 1 Derivative of a Likelihood

Recall that the likelihood function is viewed as a function of the parameters  $\theta$  and the data  $y$  are considered fixed. Thus, when we take the derivative of the log-likelihood function, it is with respect to  $\theta$  only.

**Example:** Consider the normal likelihood where only the mean  $\mu$  is unknown:

$$\begin{aligned} f(\mathbf{y}|\mu) &= \prod_{i=1}^n \frac{1}{\sqrt{2\pi\sigma^2}} \exp \left[ -\frac{1}{2\sigma^2} (y_i - \mu)^2 \right] \\ &= \frac{1}{(\sqrt{2\pi\sigma^2})^n} \exp \left[ -\frac{1}{2\sigma^2} \sum_{i=1}^n (y_i - \mu)^2 \right] \end{aligned}$$

which yields the log-likelihood

$$\begin{aligned} \ell(\mu) &= -\frac{n}{2} \log(2\pi\sigma^2) - \frac{1}{2\sigma^2} \sum_{i=1}^n (y_i - \mu)^2 \\ &= -\frac{n}{2} \log(2\pi\sigma^2) - \frac{1}{2\sigma^2} \left[ \sum_{i=1}^n (y_i^2 - 2\mu y_i + \mu^2) \right] \\ &= -\frac{n}{2} \log(2\pi\sigma^2) - \frac{1}{2\sigma^2} \left[ \sum_{i=1}^n y_i^2 - 2\mu \sum_{i=1}^n y_i + n\mu^2 \right]. \end{aligned}$$

We take the derivative of  $\ell(\mu)$  with respect to  $\mu$  to obtain

$$\begin{aligned} \frac{d\ell(\mu)}{d\mu} &= \frac{2 \sum_{i=1}^n y_i}{2\sigma^2} - \frac{2n\mu}{2\sigma^2} \\ &= \frac{\sum_{i=1}^n y_i}{\sigma^2} - \frac{n\mu}{\sigma^2}. \end{aligned} \tag{1}$$

If we set the expression in (1) equal to 0, we obtain the MLE  $\hat{\mu} = \frac{1}{n} \sum_{i=1}^n y_i = \bar{y}$ .

## 2 Products of Indicator Functions

Because  $0 \cdot 1 = 0$ , the product of indicator functions can be combined into a single indicator function with a modified condition.

**Examples:**  $I_{\{x < 5\}} \cdot I_{\{x \geq 0\}} = I_{\{0 \leq x < 5\}}$ , and  $\prod_{i=1}^n I_{\{x_i < 2\}} = I_{\{x_i < 2 \text{ for all } i\}} = I_{\{\max_i x_i < 2\}}$ .